Wavelet/Determinacy/Convert.lean
@@ -1,4 +1,5 @@
 import Wavelet.Determinacy.Defs
+import Wavelet.Determinacy.Determinism
 
 /-! Conversion between various stepping relations. -/
 
@@ -15,12 +16,11 @@ theorem Config.IdxGuardStep.to_guarded
   {ioSpec : IOSpec V T m n}
   {s s' : ConfigWithSpec opSpec χ m n}
   {l : Label Op V m n}
-  (hl : l.isYield ∨ l.isSilent)
   (hstep : Config.IdxGuardStep opSpec ioSpec s (i, l) s') :
     (Config.GuardStep opSpec ioSpec) s l s'
   := by
   rcases hstep with ⟨⟨hguard⟩, hstep⟩
-  cases hguard <;> simp at hl
+  cases hguard
   case spec_yield =>
     have := Config.IndexedStep.to_step_yield_or_tau hstep
     exact .step .spec_yield this
@@ -30,6 +30,7 @@ theorem Config.IdxGuardStep.to_guarded
   case spec_tau =>
     have := Config.IndexedStep.to_step_yield_or_tau hstep
     exact .step .spec_tau this
+  any_goals cases hstep
 
 /-- Converts a guarded step to an indexed guarded step. -/
 theorem Config.GuardStep.to_indexed_guarded
@@ -58,18 +59,17 @@ theorem Config.GuardStep.to_indexed_guarded
 
 /-- Converts an indexed unguarded step to an unguarded step. -/
 theorem Config.IdxTrivStep.to_unguarded
-  [Arity Op] [PCM T]
+  [Arity Op]
   [DecidableEq χ]
   [InterpConsts V]
   {opSpec : OpSpec Op V T}
   {s s' : ConfigWithSpec opSpec χ m n}
   {l : Label Op V m n}
-  (hl : l.isYield ∨ l.isSilent)
   (hstep : Config.IdxTrivStep opSpec s (i, l) s') :
     Config.TrivStep opSpec s l s'
   := by
   rcases hstep with ⟨⟨hguard⟩, hstep⟩
-  cases hguard <;> simp at hl
+  cases hguard
   case triv_yield =>
     have := Config.IndexedStep.to_step_yield_or_tau hstep
     exact .step .triv_yield this
@@ -79,10 +79,11 @@ theorem Config.IdxTrivStep.to_unguarded
   case triv_tau =>
     have := Config.IndexedStep.to_step_yield_or_tau hstep
     exact .step .triv_tau this
+  any_goals cases hstep
 
 /-- Converts an unguarded step to an indexed unguarded step. -/
 theorem Config.TrivStep.to_indexed_unguarded
-  [Arity Op] [PCM T]
+  [Arity Op]
   [DecidableEq χ]
   [InterpConsts V]
   {opSpec : OpSpec Op V T}
@@ -139,5 +140,129 @@ theorem Config.IdxInterpGuardStep.to_indexed_interp_unguarded_star
   (htrace : (Config.IdxInterpGuardStep opSpec ioSpec).Star s tr s') :
     (Config.IdxInterpTrivStep opSpec).Star s tr s'
   := htrace.map_step Config.IdxInterpGuardStep.to_indexed_interp_unguarded
+
+theorem Config.IdxInterpGuardStep.to_interp_guarded
+  [Arity Op] [PCM T]
+  [DecidableEq χ]
+  [InterpConsts V]
+  [opInterp : OpInterp Op V]
+  {opSpec : OpSpec Op V T}
+  {ioSpec : IOSpec V T m n}
+  {s s' : ConfigWithSpec opSpec χ m n × opInterp.S}
+  (hstep : Config.IdxInterpGuardStep opSpec ioSpec s (i, l) s') :
+    Config.InterpGuardStep opSpec ioSpec s l s'
+  := hstep.to_interp Config.IdxGuardStep.to_guarded
+
+theorem Config.IdxInterpGuardStep.to_interp_guarded_tau_star
+  [Arity Op] [PCM T]
+  [DecidableEq χ]
+  [InterpConsts V]
+  [opInterp : OpInterp Op V]
+  {opSpec : OpSpec Op V T}
+  {ioSpec : IOSpec V T m n}
+  {s s' : ConfigWithSpec opSpec χ m n × opInterp.S}
+  (htrace : (Config.IdxInterpGuardStep opSpec ioSpec).Star s tr s') :
+    (Config.InterpGuardStep opSpec ioSpec).TauStarN .τ tr.length s s'
+  := by
+  induction htrace with
+  | refl => exact .refl
+  | tail pref tail ih =>
+    have := tail.to_interp_guarded
+    have hl := proc_indexed_interp_guarded_step_label tail
+    simp [hl] at this
+    simp
+    exact .tail ih this
+
+theorem Config.InterpGuardStep.to_indexed_interp_guarded_tau
+  [Arity Op] [PCM T]
+  [DecidableEq χ]
+  [InterpConsts V]
+  [opInterp : OpInterp Op V]
+  {opSpec : OpSpec Op V T}
+  {ioSpec : IOSpec V T m n}
+  {s s' : ConfigWithSpec opSpec χ m n × opInterp.S}
+  (hstep : Config.InterpGuardStep opSpec ioSpec s .τ s') :
+    ∃ i, Config.IdxInterpGuardStep opSpec ioSpec s (i, .τ) s'
+  := hstep.to_indexed_interp_tau Config.GuardStep.to_indexed_guarded
+
+theorem Config.InterpGuardStep.to_indexed_interp_guarded_tau_star
+  [Arity Op] [PCM T]
+  [DecidableEq χ]
+  [InterpConsts V]
+  [opInterp : OpInterp Op V]
+  {opSpec : OpSpec Op V T}
+  {ioSpec : IOSpec V T m n}
+  {s s' : ConfigWithSpec opSpec χ m n × opInterp.S}
+  (htrace : (Config.InterpGuardStep opSpec ioSpec).TauStarN .τ k s s') :
+    ∃ tr,
+      tr.length = k ∧
+      (Config.IdxInterpGuardStep opSpec ioSpec).Star s tr s'
+  := by
+  induction htrace with
+  | refl => exact ⟨_, by simp, .refl⟩
+  | tail pref tail ih =>
+    have ⟨_, h, pref'⟩ := ih
+    have ⟨_, hstep'⟩ := tail.to_indexed_interp_guarded_tau
+    exact ⟨_, by simp [h], .tail pref' hstep'⟩
+
+theorem Config.IdxInterpTrivStep.to_interp_unguarded
+  [Arity Op]
+  [DecidableEq χ]
+  [InterpConsts V]
+  [opInterp : OpInterp Op V]
+  {opSpec : OpSpec Op V T}
+  {s s' : ConfigWithSpec opSpec χ m n × opInterp.S}
+  (hstep : Config.IdxInterpTrivStep opSpec s (i, l) s') :
+    Config.InterpTrivStep opSpec s l s'
+  := hstep.to_interp Config.IdxTrivStep.to_unguarded
+
+theorem Config.IdxInterpTrivStep.to_interp_unguarded_tau_star
+  [Arity Op]
+  [DecidableEq χ]
+  [InterpConsts V]
+  [opInterp : OpInterp Op V]
+  {opSpec : OpSpec Op V T}
+  {s s' : ConfigWithSpec opSpec χ m n × opInterp.S}
+  (htrace : (Config.IdxInterpTrivStep opSpec).Star s tr s') :
+    (Config.InterpTrivStep opSpec).TauStarN .τ tr.length s s'
+  := by
+  induction htrace with
+  | refl => exact .refl
+  | tail pref tail ih =>
+    have := tail.to_interp_unguarded
+    have hl := proc_indexed_interp_unguarded_step_label tail
+    simp [hl] at this
+    simp
+    exact .tail ih this
+
+theorem Config.InterpTrivStep.to_indexed_interp_unguarded_tau
+  [Arity Op]
+  [DecidableEq χ]
+  [InterpConsts V]
+  [opInterp : OpInterp Op V]
+  {opSpec : OpSpec Op V T}
+  {s s' : ConfigWithSpec opSpec χ m n × opInterp.S}
+  (hstep : Config.InterpTrivStep opSpec s .τ s') :
+    ∃ i, Config.IdxInterpTrivStep opSpec s (i, .τ) s'
+  := hstep.to_indexed_interp_tau Config.TrivStep.to_indexed_unguarded
+
+theorem Config.InterpTrivStep.to_indexed_interp_unuarded_tau_star
+  [Arity Op]
+  [DecidableEq χ]
+  [InterpConsts V]
+  [opInterp : OpInterp Op V]
+  {opSpec : OpSpec Op V T}
+  {s s' : ConfigWithSpec opSpec χ m n × opInterp.S}
+  (htrace : (Config.InterpTrivStep opSpec).TauStarN .τ k s s') :
+    ∃ tr,
+      tr.length = k ∧
+      (Config.IdxInterpTrivStep opSpec).Star s tr s'
+  := by
+  induction htrace with
+  | refl => exact ⟨_, by simp, .refl⟩
+  | tail pref tail ih =>
+    have ⟨_, h, pref'⟩ := ih
+    have ⟨_, hstep'⟩ := tail.to_indexed_interp_unguarded_tau
+    exact ⟨_, by simp [h], .tail pref' hstep'⟩
 
 end Wavelet.Dataflow
